Prove that the LR is a PER

typing.v
@@ -1,5 +1,5 @@
 Require Export syntax ssrbool ssreflect.
-From Hammer Require Import Tactics.
+From Hammer Require Import Tactics Hammer.
 
 Definition context n := fin n -> ty.
 
@@ -90,27 +90,44 @@ Inductive Reds {n} (Γ : context n) (a : tm n) : tm n -> ty -> Prop :=
   Γ ⊢ a ⤳* a ∈ A
 | Rs_Step b c A :
   Γ ⊢ a ⤳ b ∈ A ->
-  Γ ⊢ b ∈ A ->
   Γ ⊢ b ⤳* c ∈ A ->
   Γ ⊢ a ⤳* c ∈ A
 where "Γ ⊢ a ⤳* b ∈ A" := (Reds Γ a b A).
+
+Fixpoint ne {n} (a : tm n) :=
+  match a with
+  | var_tm _ => true
+  | App a b => ne a
+  | Lam _ _ => false
+  | TmUnit => false
+  | TmK => false
+  end.
 
 Definition ren_ok {n m} ξ (Γ : context n) (Δ : context m) :=
   forall i, Γ i = Δ (ξ i).
 
 Fixpoint LR {n} (Γ : context n) (b0 b1 : tm n) (A : ty) : Prop :=
   match A with
-  | TyUnit => Γ ⊢ b0 ∈ TyUnit /\ Γ ⊢ b1 ∈ TyUnit
-  | Fun A B => Γ ⊢ b0 ≡ b1 ∈ Fun A B /\
+  | TyUnit => exists a0 a1, Γ ⊢ b0 ⤳* a0 ∈ TyUnit /\ Γ ⊢ b1 ⤳* a1 ∈ TyUnit /\
+                        (ne a0 \/ a0 = TmUnit) /\ (ne a1 \/ a1 = TmUnit)
+  | Fun A B => Γ ⊢ b0 ∈ Fun A B /\ Γ ⊢ b1 ∈ Fun A B /\ Γ ⊢ b0 ≡ b1 ∈ Fun A B /\
                 forall m ξ (Δ : context m), ren_ok ξ Γ Δ ->
                          forall a0 a1, LR Δ a0 a1 A -> LR Δ (App (ren_tm ξ b0) a0) (App (ren_tm ξ b1) a1) B
-  | _ => Γ ⊢ b0 ≡ b1 ∈ A
+  | _ => False
   end.
 
+Lemma red_wt_l n (Γ : context n) (a b : tm n) (A : ty)
+  (h : Γ ⊢ a ⤳ b ∈ A) : Γ ⊢ a ∈ A.
+Proof. elim : a b A /h; hauto lq:on ctrs:DEquiv, Wt. Qed.
+
+Lemma reds_wt_l n (Γ : context n) (a b : tm n) (A : ty)
+  (h : Γ ⊢ a ⤳* b ∈ A) : Γ ⊢ a ∈ A.
+Proof. elim : a b A /h; hauto lq:on use:red_wt_l ctrs:DEquiv, Wt. Qed.
+
 Lemma escape {n} (Γ : context n) (a b : tm n) (A : ty) :
-  LR Γ a b A -> Γ ⊢ a ≡ b ∈ A.
+  LR Γ a b A -> Γ ⊢ a ≡ b ∈ A /\ Γ ⊢ a ∈ A /\ Γ ⊢ b ∈ A.
 Proof.
-  elim : A n Γ a b=> //=; hauto lq:on ctrs:DEquiv.
+  elim : A n Γ a b=> //=; hauto l:on use:reds_wt_l ctrs:DEquiv, Wt.
 Qed.
 
 Definition subst_ok {n m}
@@ -121,14 +138,73 @@ Definition subst_ok {n m}
 
 Definition SEquiv {n} (Γ : context n) (b0 b1 : tm n) (A : ty) :=
   forall m ρ δ (Δ : context m), subst_ok ρ δ Γ Δ ->
-                              LR Δ (subst_tm ρ b0) (subst_tm ρ b1) A.
+                              LR Δ (subst_tm ρ b0) (subst_tm δ b1) A.
 
 Notation "Γ ⊨ b0 ≡ b1 ∈ A" := (SEquiv Γ b0 b1 A) (at level 70, no associativity).
+
+Lemma lr_sym n (Γ : context n) (b0 b1 : tm n) (A : ty) :
+  LR Γ b0 b1 A -> LR Γ b1 b0 A.
+Proof.
+  elim : A n Γ b0 b1=>//=; qauto l:on ctrs:Wt, DEquiv.
+Qed.
+
+Lemma lr_trans n (Γ : context n) (b0 b1 b2 : tm n) (A : ty) :
+  LR Γ b0 b1 A -> LR Γ b1 b2 A -> LR Γ b0 b2 A.
+Proof.
+  elim : A n Γ b0 b1 b2 => //=.
+  - move => A ihA B ihB n Γ b0 b1 b2 [h00 h01] [h10 h11].
+    repeat split=> /ltac:(try tauto);  first by hauto lq:on ctrs:DEquiv.
+    move {h00 h10}.
+    move => m ξ Δ h a0 a1 ha.
+    have : LR Δ a1 a1 A by hauto lq:on use:lr_sym.
+    qauto l:on.
+  - hauto lq:on.
+Qed.
+
+Lemma lr_left_right_refl n (Γ : context n) a0 a1 A :
+  LR Γ a0 a1 A -> LR Γ a0 a0 A /\ LR Γ a1 a1 A.
+Proof. hauto lq:on use:lr_sym, lr_trans. Qed.
+
+Lemma ren_ok_id {n} (Γ : context n) :
+  ren_ok id Γ Γ.
+Proof. sfirstorder. Qed.
+
+Lemma lr_back_clos_left : forall A n (Γ : context n) a0 b0 a1,
+    Γ ⊢ a1 ⤳ a0 ∈ A ->
+    LR Γ a0 b0 A ->
+    LR Γ a1 b0 A.
+Proof.
+  elim => //=.
+  - move => A ihA B ihB n Γ a0 b0 a1 h [h00 h01].
+    repeat split.
+    + sfirstorder use:red_wt_l.
+    + sfirstorder.
+    + admit.
+    + move => m ξ Δ hξ c0 c1 hc.
+      suff : Δ ⊢ App (ren_tm ξ a1) c0 ⤳ App (ren_tm ξ a0) c0 ∈ B by sfirstorder.
+      apply R_App with (A := A); last by hauto lq:on use:escape.
+      admit.
+  - hauto lq:on ctrs:Reds.
+Admitted.
 
 Lemma soundness {n} (Γ : context n) a A : Γ ⊢ a ∈ A -> Γ ⊨ a ≡ a ∈ A.
 Proof.
   move => h.
   elim : n Γ a A / h.
-  - rewrite /SEquiv.
-    simpl.
+  - hauto l:on use:lr_left_right_refl unfold:SEquiv.
+  - rewrite /SEquiv => n Γ A b B hb ihb m ρ δ Δ hδρ /=.
+    split.
+    + admit.
+    + move => p ξ Ψ hξ a0 a1 ha.
+      asimpl.
+
+  - move => n Γ A B b a hb ihb ha iha m ρ δ Δ hρδ //=.
+    rewrite /SEquiv in ihb iha.
+    move : ihb (hρδ) => /[apply].
+    move : iha (hρδ) => /[apply] /=.
+    move => iha [ihb0 ihb1].
+    move : ihb1 (ren_ok_id Δ)  => /[apply].
+    asimpl.
+    by apply.
+  - hauto l:on.
 Admitted.
